Add some new theorems.  In particular, an induction principle for proving goals of the form !l1 l2. PERM l1 l2 ==> P l1 l2.   Also rename PERM_TRANS1 to PERM_TRANS, and PERM_TRANS to PERM_transitive. x_TRANS is used elsewhere for theorems of the form   R x y /\ R y z ==> R x z so this feels more consistent.

src/sort/sortingScript.sml
@@ -9,8 +9,10 @@ struct
 app load ["permTheory","bossLib"];
 *)
 
-open HolKernel Parse boolLib bossLib 
-     combinTheory pairTheory relationTheory listTheory;
+open HolKernel Parse boolLib bossLib
+
+open combinTheory pairTheory relationTheory listTheory metisLib
+     BasicProvers
 
 
 val _ = new_theory "sorting";
@@ -32,6 +34,7 @@ val PERM_REFL = Q.store_thm
 ("PERM_REFL",
     `!L. PERM L L`,
     PROVE_TAC[PERM_DEF]);
+val _ = export_rewrites ["PERM_REFL"]
 
 
 val PERM_INTRO = Q.store_thm
@@ -40,17 +43,16 @@ val PERM_INTRO = Q.store_thm
     PROVE_TAC[PERM_REFL]);
 
 
-val PERM_TRANS = Q.store_thm
-("PERM_TRANS",
+val PERM_transitive = Q.store_thm
+("PERM_transitive",
   `transitive PERM`,
- RW_TAC list_ss [relationTheory.transitive_def] 
+ RW_TAC list_ss [relationTheory.transitive_def]
   THEN PROVE_TAC[PERM_DEF]);
 
-
-val PERM_TRANS1 = save_thm
-("PERM_TRANS1",
- REWRITE_RULE [relationTheory.transitive_def] PERM_TRANS);
-
+val PERM_TRANS = Q.store_thm
+("PERM_TRANS",
+ `!x y z. PERM x y /\ PERM y z ==> PERM x z`,
+ METIS_TAC [relationTheory.transitive_def, PERM_transitive])
 
 val PERM_SYM = Q.store_thm
 ("PERM_SYM",
@@ -59,8 +61,8 @@ PROVE_TAC [PERM_DEF]);
 
 val PERM_CONG = Q.store_thm
 ("PERM_CONG",
- `!(L1:'a list) L2 L3 L4. 
-     PERM L1 L3 /\ 
+ `!(L1:'a list) L2 L3 L4.
+     PERM L1 L3 /\
      PERM L2 L4
      ==> PERM (APPEND L1 L2) (APPEND L3 L4)`,
  PROVE_TAC [PERM_DEF,FILTER_APPEND_DISTRIB]);
@@ -73,104 +75,262 @@ val PERM_MONO = Q.store_thm
  PROVE_TAC [CONS_APPEND,PERM_CONG, PERM_REFL]);
 
 
-val PERM_CONS_IFF = 
+val PERM_CONS_IFF =
 let val lem = Q.prove
      (`PERM (x::l1) (x::l2) ==> PERM l1 l2`,
       RW_TAC list_ss [PERM_DEF,FILTER]
         THEN POP_ASSUM (MP_TAC o Q.SPEC`x'`)
         THEN RW_TAC list_ss [])
-in 
+in
   save_thm ("PERM_CONS_IFF",
             GEN_ALL(IMP_ANTISYM_RULE lem (SPEC_ALL PERM_MONO)))
 end;
 
+val _ = export_rewrites ["PERM_CONS_IFF"]
+
 val PERM_NIL = Q.store_thm
 ("PERM_NIL",
- `!L. (PERM L [] = (L=[])) /\ 
+ `!L. (PERM L [] = (L=[])) /\
       (PERM [] L = (L=[]))`,
 Cases THEN RW_TAC list_ss [PERM_DEF,FILTER]
  THEN Q.EXISTS_TAC `h`
  THEN RW_TAC list_ss []);
 
+val _ = export_rewrites ["PERM_NIL"]
 
-val lem = Q.prove(
- `!h l1 l2. APPEND (FILTER ($=h) l1) (h::l2)
-            = h::APPEND (FILTER ($=h) l1) l2`,
-Induct_on `l1` 
-   THEN RW_TAC list_ss [FILTER] 
-   THEN PROVE_TAC[]);
+val PERM_SING = Q.store_thm
+("PERM_SING",
+ `(PERM L [x] = (L = [x])) /\ (PERM [x] L = (L = [x]))`,
+ Q_TAC SUFF_TAC `PERM L [x] = (L = [x])`
+       THEN1 METIS_TAC [PERM_SYM] THEN
+ Cases_on `L` THEN SIMP_TAC (srw_ss()) [PERM_DEF, EQ_IMP_THM] THEN
+ Q_TAC SUFF_TAC
+       `(!y. (if y = h then h :: FILTER ($= h) t else FILTER ($= y) t) =
+             (if y = x then [x] else [])) ==>
+        (h = x) /\ (t = [])`
+       THEN1 METIS_TAC [] THEN
+ STRIP_TAC THEN
+ `h = x` by (POP_ASSUM (Q.SPEC_THEN `h` MP_TAC) THEN SRW_TAC [][]) THEN
+ SRW_TAC [][] THEN
+ `!y. FILTER ($= y) t = []` by METIS_TAC [CONS_11] THEN
+ Cases_on `t` THEN FULL_SIMP_TAC (srw_ss()) [] THEN
+ METIS_TAC [NOT_CONS_NIL]);
+val _ = export_rewrites ["PERM_SING"]
 
+val MEM_FILTER_EQ = Q.prove
+(`!l x. MEM x l = ~(FILTER ($= x) l = [])`,
+ Induct THEN SRW_TAC [][]);
+
+val MEM_APPEND_SPLIT = Q.prove
+(`!L x. MEM x L ==> ?M N. L = M ++ x::N`,
+ Induct THEN SRW_TAC [][] THENL [
+   Q.EXISTS_TAC `[]` THEN SRW_TAC [][],
+   `?M N. L = M ++ x::N` by METIS_TAC [] THEN
+   Q.EXISTS_TAC `h::M` THEN SRW_TAC [][]
+ ]);
+
+val FILTER_EQ_CONS_APPEND = Q.prove
+(`!M N x. FILTER ($= x) M ++ x::N = x::FILTER ($= x) M ++ N`,
+ Induct THEN SRW_TAC [][])
+
+val PERM_CONS_EQ_APPEND = Q.store_thm
+("PERM_CONS_EQ_APPEND",
+ `!L h. PERM (h::t) L = ?M N. (L = M ++ h::N) /\ PERM t (M ++ N)`,
+ SRW_TAC [][PERM_DEF, FILTER_APPEND_DISTRIB, EQ_IMP_THM] THENL [
+   `MEM h L` by METIS_TAC [NOT_CONS_NIL, MEM_FILTER_EQ] THEN
+   `?M N. L = M ++ h::N` by METIS_TAC [MEM_APPEND_SPLIT] THEN
+   MAP_EVERY Q.EXISTS_TAC [`M`, `N`] THEN
+   SRW_TAC [][] THEN Cases_on `x = h` THEN
+   FIRST_X_ASSUM (Q.SPEC_THEN `x` MP_TAC) THEN
+   SRW_TAC [][FILTER_APPEND_DISTRIB, FILTER_EQ_CONS_APPEND],
+   SRW_TAC [][FILTER_APPEND_DISTRIB, FILTER_EQ_CONS_APPEND]
+ ]);
 
 val PERM_APPEND = Q.store_thm
 ("PERM_APPEND",
  `!l1 l2. PERM (APPEND l1 l2) (APPEND l2 l1)`,
-RW_TAC list_ss [PERM_DEF,FILTER_APPEND_DISTRIB]
-  THEN Induct_on `l1` 
-  THEN RW_TAC list_ss [FILTER,lem]
-  THEN PROVE_TAC[]);;
-
+ Induct THEN SRW_TAC [][PERM_CONS_EQ_APPEND] THEN METIS_TAC [])
 
 val CONS_PERM = Q.store_thm
 ("CONS_PERM",
- `!x L M N. PERM L (APPEND M N) 
-            ==> 
+ `!x L M N. PERM L (APPEND M N)
+            ==>
            PERM (x::L) (APPEND M (x::N))`,
-RW_TAC bool_ss []
- THEN MATCH_MP_TAC PERM_TRANS1
- THEN PROVE_TAC [PERM_MONO, PERM_APPEND, APPEND, PERM_TRANS1]);
+METIS_TAC [PERM_CONS_EQ_APPEND]);
 
 
 val APPEND_PERM_SYM = Q.store_thm
 ("APPEND_PERM_SYM",
  `!A B C. PERM (APPEND A B) C ==> PERM (APPEND B A) C`,
-PROVE_TAC [PERM_TRANS1, PERM_APPEND]);
+PROVE_TAC [PERM_TRANS, PERM_APPEND]);
 
 val PERM_SPLIT = Q.store_thm
 ("PERM_SPLIT",
  `!P l. PERM l (APPEND (FILTER P l) (FILTER ($~ o P) l))`,
 RW_TAC bool_ss [o_DEF]
  THEN Induct_on `l`
- THEN RW_TAC list_ss [FILTER,PERM_REFL] 
+ THEN RW_TAC list_ss [FILTER,PERM_REFL]
  THEN PROVE_TAC [APPEND,PERM_MONO,CONS_PERM]);
 
+(* ----------------------------------------------------------------------
+    Inductive characterisation of PERM
+   ---------------------------------------------------------------------- *)
 
-(*---------------------------------------------------------------------------
-    Directly performs one "sorting step" between 2 non-empty lists that 
-    are permutations of each other.
- *---------------------------------------------------------------------------*)
+(* things become slightly awkward because I avoid actually defining an
+   inductive version of the permutation constant.  Instead, I do a bunch
+   of proofs subject to an assumption "defining" perm to be the
+   appropriate RHS; an alernative would be to define the constant, work
+   with it, and then to delete it, so that it didn't get exported. *)
 
-val PERM_SORT_STEP = Q.store_thm
-("PERM_SORT_STEP",
- `!l h t. PERM (h::t) l ==> ?rst. h::rst = FILTER ($=h) l`,
- RW_TAC list_ss [PERM_DEF,FILTER] 
-   THEN POP_ASSUM (MP_TAC o Q.SPEC`h`)
-   THEN RW_TAC bool_ss []
-   THEN PROVE_TAC[]);
+(* the definition assumption is 'backwards' so that it will be OK as an
+   assumption and not cause perm to get rewritten out *)
+val perm_t =
+  ``!l1 l2:'a list. (!P. P [] [] /\
+                         (!x l1 l2. P l1 l2 ==> P (x::l1) (x::l2)) /\
+                         (!x y l1 l2. P l1 l2 ==> P (x::y::l1) (y::x::l2)) /\
+                         (!l1 l2 l3. P l1 l2 /\ P l2 l3 ==> P l1 l3) ==>
+                         P l1 l2) = perm l1 l2``
 
-val LENGTH_APPEND_FILTER = Q.prove
-(`!L. LENGTH L = LENGTH (APPEND (FILTER P L) (FILTER ($~ o P) L))`,
-Induct 
- THEN RW_TAC list_ss [FILTER, o_DEF] 
- THEN PROVE_TAC []);
+(* perm's induction principle *)
+val _ = print "Proving perm induction principle\n"
+val perm_ind = prove(
+  ``^perm_t ==> !P. P [] [] /\
+                    (!x l1 l2. P l1 l2 ==> P (x::l1) (x::l2)) /\
+                    (!x y l1 l2. P l1 l2 ==> P (x::y::l1) (y::x::l2)) /\
+                    (!l1 l2 l3. P l1 l2 /\ P l2 l3 ==> P l1 l3) ==>
+                    !l1 l2. perm l1 l2 ==> P l1 l2``,
+  DISCH_THEN (fn th => REWRITE_TAC [GSYM th]) THEN REPEAT STRIP_TAC THEN
+  FIRST_ASSUM MATCH_MP_TAC THEN ASM_REWRITE_TAC []);
+val perm_ind = UNDISCH perm_ind
 
-val PERM_STEP = Q.prove
-(`!l h t. PERM (h::t) l 
-            ==> 
-          ?u. PERM l (h::u) /\ (LENGTH l = LENGTH (h::u))`,
-RW_TAC bool_ss []
-  THEN IMP_RES_TAC PERM_SORT_STEP
-  THEN Q.EXISTS_TAC `APPEND rst (FILTER ($~ o $= h) l)`
-  THEN PROVE_TAC [APPEND, LENGTH_APPEND_FILTER,PERM_SPLIT]);
+val _ = print "Proving perm rules\n"
+val perm_rules = prove(
+  ``^perm_t ==> perm [] [] /\
+                (!x l1 l2. perm l1 l2 ==> perm (x::l1) (x::l2)) /\
+                (!x y l1 l2. perm l1 l2 ==> perm (x::y::l1) (y::x::l2)) /\
+                (!l1 l2 l3. perm l1 l2 /\ perm l2 l3 ==> perm l1 l3)``,
+  DISCH_THEN (REWRITE_TAC o C cons nil o GSYM) THEN REPEAT STRIP_TAC THENL [
+    `P l1 l2` by RES_TAC THEN METIS_TAC [],
+    `P l1 l2` by RES_TAC THEN METIS_TAC [],
+    `P l1 l2 /\ P l2 l3` by RES_TAC THEN METIS_TAC []
+  ]);
+val perm_rules = UNDISCH perm_rules
 
+val perm_sym = prove(
+  ``^perm_t ==> (perm l1 l2 = perm l2 l1)``,
+  STRIP_TAC THEN
+  Q_TAC SUFF_TAC
+        `!l1 l2. perm l1 l2 ==> perm l2 l1`
+        THEN1 mesonLib.MESON_TAC [] THEN
+  HO_MATCH_MP_TAC perm_ind THEN
+  SRW_TAC [][perm_rules] THEN METIS_TAC [perm_rules]);
+val perm_sym = UNDISCH perm_sym
+
+val perm_refl = prove(
+  ``^perm_t ==> !l. perm l l``,
+  STRIP_TAC THEN Induct THEN SRW_TAC [][perm_rules]);
+val perm_refl = UNDISCH perm_refl
+
+val perm_trans = last (CONJUNCTS perm_rules)
+val _ = print "Proving perm symmetric, reflexive & transitive\n"
+
+val perm_PERM = prove(
+  ``^perm_t ==> !l1 l2. perm l1 l2 ==> PERM l1 l2``,
+  STRIP_TAC THEN HO_MATCH_MP_TAC perm_ind THEN
+  SRW_TAC [][] THENL [
+    SRW_TAC [][PERM_CONS_EQ_APPEND] THEN
+    MAP_EVERY Q.EXISTS_TAC [`[y]`, `l2`] THEN SRW_TAC [][] THEN
+    MAP_EVERY Q.EXISTS_TAC [`[]`, `l2`] THEN SRW_TAC [][],
+    METIS_TAC [PERM_TRANS]
+  ]);
+val perm_PERM = UNDISCH perm_PERM
+
+val _ = print "Proving perm has primitive recursive characterisation\n"
+val perm_cons_append = prove(
+  ``^perm_t ==> !l1 l2. perm l1 l2 ==>
+                        !M N. (l2 = M ++ N) ==>
+                              !h. perm (h::l1) (M ++ h::N)``,
+  STRIP_TAC THEN HO_MATCH_MP_TAC perm_ind THEN SRW_TAC [][] THENL [
+    SRW_TAC [][perm_rules],
+    Cases_on `M` THEN SRW_TAC [][] THENL [
+      FULL_SIMP_TAC (srw_ss()) [] THEN SRW_TAC [][] THEN
+      FIRST_X_ASSUM (Q.SPECL_THEN [`[]`, `l2`] MP_TAC) THEN
+      SRW_TAC [][] THEN METIS_TAC [perm_rules],
+      FULL_SIMP_TAC (srw_ss()) [] THEN SRW_TAC [][] THEN
+      MATCH_MP_TAC perm_trans THEN
+      Q.EXISTS_TAC `h'::h::l1` THEN SRW_TAC [][perm_rules, perm_refl]
+    ],
+    `(M = []) \/ (?m1 ms. M = m1::ms)` by (Cases_on `M` THEN SRW_TAC [][]) THEN
+    SRW_TAC [][] THEN FULL_SIMP_TAC (srw_ss()) [] THEN SRW_TAC [][] THENL [
+      MATCH_MP_TAC perm_trans THEN
+      Q.EXISTS_TAC `h::y::x::l1` THEN
+      FIRST_X_ASSUM (Q.SPECL_THEN [`[]`, `l2`] MP_TAC) THEN
+      SRW_TAC [][perm_rules, perm_refl],
+      `(ms = []) \/ (?m2 mss. ms = m2::mss)`
+          by (Cases_on `ms` THEN SRW_TAC [][]) THEN
+      SRW_TAC [][] THEN FULL_SIMP_TAC (srw_ss()) [] THEN SRW_TAC [][] THENL [
+        FIRST_X_ASSUM (Q.SPECL_THEN [`[]`, `l2`] MP_TAC) THEN
+        SRW_TAC [][] THEN
+        MATCH_MP_TAC perm_trans THEN
+        Q.EXISTS_TAC `h::m1::x::l1` THEN SRW_TAC [][perm_rules,perm_refl],
+        FIRST_X_ASSUM (Q.SPECL_THEN [`mss`, `N`] MP_TAC) THEN
+        SRW_TAC [][] THEN MATCH_MP_TAC perm_trans THEN
+        Q.EXISTS_TAC `m2::h::m1::l1` THEN
+        SRW_TAC [][perm_rules, perm_refl] THEN
+        MATCH_MP_TAC perm_trans THEN Q.EXISTS_TAC `m2::m1::h::l1` THEN
+        SRW_TAC [][perm_rules, perm_refl]
+      ]
+    ],
+    `!h. perm (h::l1) (h::l1')` by METIS_TAC [APPEND] THEN
+    METIS_TAC [perm_trans]
+  ])
+val perm_cons_append =
+    SIMP_RULE (bool_ss ++ boolSimps.DNF_ss) [] (UNDISCH perm_cons_append)
+
+val PERM_perm = prove(
+  ``^perm_t ==> !l1 l2. PERM l1 l2 ==> perm l1 l2``,
+  STRIP_TAC THEN Induct THEN SRW_TAC [][perm_rules, PERM_CONS_EQ_APPEND] THEN
+  METIS_TAC [perm_cons_append])
+val PERM_perm = UNDISCH PERM_perm
+
+
+val perm_elim = GEN_ALL
+                  (IMP_ANTISYM_RULE (SPEC_ALL perm_PERM) (SPEC_ALL PERM_perm))
+fun remove_eq_asm th = let
+  val th0 =
+      CONV_RULE (LAND_CONV (SIMP_CONV (bool_ss ++ boolSimps.ETA_ss)
+                                      [GSYM FUN_EQ_THM]))
+                (DISCH_ALL (REWRITE_RULE [perm_elim] th))
+in
+  CONV_RULE Unwind.UNWIND_FORALL_CONV
+            (GEN ``perm : 'a list -> 'a list -> bool`` th0)
+end
+
+val PERM_IND = save_thm("PERM_IND", remove_eq_asm perm_ind)
+
+val PERM_SWAP_AT_FRONT = store_thm(
+  "PERM_SWAP_AT_FRONT",
+  ``PERM (x::y::l1) (y::x::l2) = PERM l1 l2``,
+  METIS_TAC [remove_eq_asm (List.nth(CONJUNCTS perm_rules, 2)),
+             PERM_REFL, PERM_TRANS, PERM_CONS_IFF]);
 
 val PERM_LENGTH = Q.store_thm("PERM_LENGTH",
 `!l1 l2. PERM l1 l2 ==> (LENGTH l1 = LENGTH l2)`,
-Induct 
-  THEN RW_TAC list_ss [PERM_NIL]
-  THEN IMP_RES_TAC PERM_STEP
-  THEN `PERM l1 u` by PROVE_TAC [PERM_TRANS1,PERM_CONS_IFF]
-  THEN RW_TAC list_ss []);
+HO_MATCH_MP_TAC PERM_IND THEN SRW_TAC [][])
 
+(*---------------------------------------------------------------------------
+    Directly performs one "sorting step" between 2 non-empty lists that
+    are permutations of each other.
+ *---------------------------------------------------------------------------*)
+
+(* unused? *)
+val PERM_SORT_STEP = Q.store_thm
+("PERM_SORT_STEP",
+ `!l h t. PERM (h::t) l ==> ?rst. h::rst = FILTER ($=h) l`,
+ RW_TAC list_ss [PERM_DEF,FILTER]
+   THEN POP_ASSUM (MP_TAC o Q.SPEC`h`)
+   THEN RW_TAC bool_ss []
+   THEN PROVE_TAC[]);
 
 (*---------------------------------------------------------------------------*
  * The idea of sortedness requires a "permutation" relation for lists, and   *
@@ -182,7 +342,7 @@ val SORTED_DEF = Define `(SORTED R [] = T) /\ (SORTED R [x] = T) /\
  (SORTED R (x::y::rst) = R x y /\ SORTED R (y::rst))`;
 
 
-val SORTS_DEF = 
+val SORTS_DEF =
  Define
     `SORTS f R = !l. PERM l (f R l) /\ SORTED R (f R l)`;
 
@@ -195,7 +355,7 @@ val SORTED_EQ = Q.store_thm
 ("SORTED_EQ",
  `!R L x. transitive R ==> (SORTED R (x::L) = SORTED R L /\ !y. MEM y L ==> R x y)`,
 Induct_on `L`
- THEN RW_TAC list_ss [SORTED_DEF,MEM] 
+ THEN RW_TAC list_ss [SORTED_DEF,MEM]
  THEN PROVE_TAC [relationTheory.transitive_def]);
 
 
@@ -204,17 +364,17 @@ Induct_on `L`
  *---------------------------------------------------------------------------*)
 
 val SORTED_APPEND = Q.store_thm("SORTED_APPEND",
-`!R L1 L2. 
-     transitive R 
+`!R L1 L2.
+     transitive R
  /\  SORTED R L1
  /\  SORTED R L2
  /\ (!x y. MEM x L1 /\ MEM y L2 ==> R x y)
-  ==> 
+  ==>
     SORTED R (APPEND L1 L2)`,
 Induct_on `L1`
- THEN RW_TAC list_ss [MEM] 
+ THEN RW_TAC list_ss [MEM]
  THEN `SORTED R L1 /\ !y. MEM y L1 ==> R h y` by PROVE_TAC [SORTED_EQ]
- THEN RW_TAC bool_ss [SORTED_EQ] 
+ THEN RW_TAC bool_ss [SORTED_EQ]
  THEN `MEM y L1 \/ MEM y L2` by PROVE_TAC [MEM_APPEND]
  THEN PROVE_TAC []);
 
@@ -223,10 +383,10 @@ Induct_on `L1`
                  Partition a list by a predicate.
  ---------------------------------------------------------------------------*)
 
-val PART_DEF = 
- Define 
+val PART_DEF =
+ Define
      `(PART P [] l1 l2 = (l1,l2))
-  /\  (PART P (h::rst) l1 l2 = 
+  /\  (PART P (h::rst) l1 l2 =
           if P h then PART P rst (h::l1) l2
                  else PART P rst  l1  (h::l2))`;
 
@@ -240,15 +400,15 @@ val PART_LENGTH = Q.store_thm
  `!P L l1 l2 p q.
     ((p,q) = PART P L l1 l2)
     ==> (LENGTH L + LENGTH l1 + LENGTH l2 = LENGTH p + LENGTH q)`,
-Induct_on `L` 
+Induct_on `L`
   THEN RW_TAC list_ss [PART_DEF]
-  THEN RES_THEN MP_TAC 
+  THEN RES_THEN MP_TAC
   THEN RW_TAC list_ss []);
 
 
 val PART_LENGTH_LEM = Q.store_thm
 ("PART_LENGTH_LEM",
-`!P L l1 l2 p q. 
+`!P L l1 l2 p q.
     ((p,q) = PART P L l1 l2)
     ==>  LENGTH p <= LENGTH L + LENGTH l1 + LENGTH l2 /\
          LENGTH q <= LENGTH L + LENGTH l1 + LENGTH l2`,
@@ -258,17 +418,17 @@ RW_TAC bool_ss []
 
 
 (*---------------------------------------------------------------------------
-     Everything in the partitions occurs in the original list, and 
-     vice-versa. The goal has been generalized. 
+     Everything in the partitions occurs in the original list, and
+     vice-versa. The goal has been generalized.
  ---------------------------------------------------------------------------*)
 
 val PART_MEM = Q.store_thm
 ("PART_MEM",
- `!P L a1 a2 l1 l2. 
-     ((a1,a2) = PART P L l1 l2) 
-       ==> 
+ `!P L a1 a2 l1 l2.
+     ((a1,a2) = PART P L l1 l2)
+       ==>
       !x. MEM x (APPEND L (APPEND l1 l2)) = MEM x (APPEND a1 a2)`,
- Induct_on `L` 
+ Induct_on `L`
   THEN RW_TAC bool_ss [PART_DEF]
   THENL [RW_TAC list_ss [], ALL_TAC, ALL_TAC]
   THEN RES_THEN MP_TAC THEN NTAC 2 (DISCH_THEN (K ALL_TAC))
@@ -276,22 +436,22 @@ val PART_MEM = Q.store_thm
   THEN RW_TAC list_ss [MEM,MEM_APPEND] THEN PROVE_TAC[]);
 
 (*---------------------------------------------------------------------------
-       Each element in the positive and negative partitions has 
-       the desired property. The simplifier loops on some of the 
+       Each element in the positive and negative partitions has
+       the desired property. The simplifier loops on some of the
        subgoals here, so we have to take round-about measures.
  ---------------------------------------------------------------------------*)
 
 val PARTS_HAVE_PROP = Q.store_thm
 ("PARTs_HAVE_PROP",
- `!P L A B l1 l2. 
+ `!P L A B l1 l2.
    ((A,B) = PART P L l1 l2) /\
    (!x. MEM x l1 ==> P x) /\ (!x. MEM x l2 ==> ~P x)
-    ==> 
+    ==>
       (!z. MEM z A ==>  P z) /\ (!z. MEM z B ==> ~P z)`,
 Induct_on `L`
  THEN REWRITE_TAC [PART_DEF,CLOSED_PAIR_EQ] THENL
  [PROVE_TAC[],
-  POP_ASSUM (fn th => REPEAT GEN_TAC THEN 
+  POP_ASSUM (fn th => REPEAT GEN_TAC THEN
      COND_CASES_TAC THEN STRIP_TAC THEN MATCH_MP_TAC th)
    THENL [MAP_EVERY Q.EXISTS_TAC [`h::l1`, `l2`],
           MAP_EVERY Q.EXISTS_TAC [`l1`, `h::l2`]]
@@ -310,14 +470,14 @@ val PART_PERM = Q.prove
    PERM (APPEND L (APPEND l1 l2)) (APPEND a1 a2)`,
 Induct_on `L`
   THEN RW_TAC list_ss [PART_DEF, PERM_REFL]
-  THEN RES_TAC THEN MATCH_MP_TAC PERM_TRANS1 THENL
+  THEN RES_TAC THEN MATCH_MP_TAC PERM_TRANS THENL
   [Q.EXISTS_TAC `APPEND L (APPEND (h::l1) l2)`,
    Q.EXISTS_TAC `APPEND L (APPEND l1 (h::l2))`]
   THEN PROVE_TAC [APPEND,APPEND_ASSOC,CONS_PERM,PERM_REFL]);
 
 (*---------------------------------------------------------------------------
-     A packaged version of PART. Most theorems about PARTITION 
-     will be instances of theorems about PART. 
+     A packaged version of PART. Most theorems about PARTITION
+     will be instances of theorems about PART.
  ---------------------------------------------------------------------------*)
 
 val PARTITION_DEF = Define`PARTITION P l = PART P l [] []`;
@@ -375,7 +535,7 @@ val QSORT_PERM = Q.store_thm
  recInduct QSORT_IND
   THEN RW_TAC bool_ss [QSORT_DEF,PERM_REFL,PARTITION_DEF]
   THEN MATCH_MP_TAC CONS_PERM
-  THEN MATCH_MP_TAC PERM_TRANS1
+  THEN MATCH_MP_TAC PERM_TRANS
   THEN Q.EXISTS_TAC`APPEND l1 l2`
   THEN RW_TAC std_ss [] THENL
   [PROVE_TAC [APPEND,APPEND_NIL,PART_PERM],
@@ -417,11 +577,11 @@ val QSORT_SORTS = Q.store_thm
 
 val _ = export_theory();
 
-val _ = 
+val _ =
  let open EmitML
  in exportML("sorting",
   [OPEN ["list"],
-   DEFN PART_DEF, 
+   DEFN PART_DEF,
    DEFN PARTITION_DEF,
    DEFN QSORT_DEF,
    DEFN SORTED_DEF])
